use one argument for contexts. also natrec.

theories/SetModel/HO.v
@@ -32,13 +32,73 @@ Proof.
     + now apply setSndPair_typing.
 Qed.
 
+(* Extended contexts *)
+
+Definition ctxExt (n : nat) (Γ : ZFSet) (A : ZFSet -> ZFSet) := setSigma n Γ (fun γ => 𝕌el n (A γ)).
+
+Definition ctx_wk (n : nat) (Γ : ZFSet) (A : ZFSet -> ZFSet) (γa : ZFSet) := setFstSigma n Γ (fun γ => 𝕌el n (A γ)) γa.
+
+Definition ctx_var0 (n : nat) (Γ : ZFSet) (A : ZFSet -> ZFSet) (γa : ZFSet) := setSndSigma n Γ (fun γ => 𝕌el n (A γ)) γa.
+
+Lemma ctx_wk_typing {n : nat} {Γ γa : ZFSet} {A : ZFSet -> ZFSet} 
+  (HA : ∀ γ ∈ Γ, A γ ∈ 𝕌 n) (Hγa : γa ∈ ctxExt n Γ A) :
+  ctx_wk n Γ A γa ∈ Γ.
+Proof.
+  apply (setFstSigma_typing (A := Γ) (B := fun γ => 𝕌el n (A γ))).
+  - intros γ Hγ. apply 𝕌el_typing. now apply HA.
+  - assumption.
+Qed.  
+
+Lemma ctx_var0_typing {n : nat} {Γ γa : ZFSet} {A : ZFSet -> ZFSet} 
+  (HA : ∀ γ ∈ Γ, A γ ∈ 𝕌 n) (Hγa : γa ∈ ctxExt n Γ A) :
+  ctx_var0 n Γ A γa ∈ 𝕌el n (A (ctx_wk n Γ A γa)).
+Proof.
+  apply (setSndSigma_typing (A := Γ) (B := fun γ => 𝕌el n (A γ))).
+  - intros γ Hγ. apply 𝕌el_typing. now apply HA.
+  - assumption.
+Qed.
+
+Lemma ctxExtβ1 {n : nat} {Γ γ a : ZFSet} {A : ZFSet -> ZFSet}
+  (HA : ∀ γ ∈ Γ, A γ ∈ 𝕌 n) (Hγ : γ ∈ Γ) (Ha : a ∈ 𝕌el n (A γ)) :
+  ctx_wk n Γ A ⟨ γ ; a ⟩ ≡ γ.
+Proof.
+  apply (setSigmaβ1 (A := Γ) (B := fun γ => 𝕌el n (A γ))) ; try assumption.
+  intros γ' Hγ'. apply 𝕌el_typing. now apply HA.
+Qed.
+
+Lemma ctxExtβ2 {n : nat} {Γ γ a : ZFSet} {A : ZFSet -> ZFSet}
+  (HA : ∀ γ ∈ Γ, A γ ∈ 𝕌 n) (Hγ : γ ∈ Γ) (Ha : a ∈ 𝕌el n (A γ)) :
+  ctx_var0 n Γ A ⟨ γ ; a ⟩ ≡ a.
+Proof.
+  apply (setSigmaβ2 (A := Γ) (B := fun γ => 𝕌el n (A γ))) ; try assumption.
+  intros γ' Hγ'. apply 𝕌el_typing. now apply HA.
+Qed.
+
+
+Lemma typeExt_typing {n : nat} {Γ γ : ZFSet} {A : ZFSet -> ZFSet} {B : ZFSet -> ZFSet}
+  (HA : ∀ γ ∈ Γ, A γ ∈ 𝕌 n) (HB : ∀ γa ∈ ctxExt n Γ A, B γa ∈ 𝕌 n) (Hγ : γ ∈ Γ) :
+  ∀ a ∈ 𝕌el n (A γ), B ⟨ γ ; a ⟩ ∈ 𝕌 n.
+Proof.
+  intros a Ha. apply HB. apply setMkSigma_typing ; try assumption.
+  clear γ Hγ a Ha. intros γ Hγ. apply 𝕌el_typing. now apply HA.
+Qed.
+
+Lemma termExt_typing {n : nat} {Γ γ : ZFSet} {A B t : ZFSet -> ZFSet} 
+  (HA : ∀ γ ∈ Γ, A γ ∈ 𝕌 n) (HB : ∀ γa ∈ ctxExt n Γ A, B γa ∈ 𝕌 n)
+  (Ht : ∀ γa ∈ ctxExt n Γ A, t γa ∈ 𝕌el n (B γa)) (Hγ : γ ∈ Γ) :
+  ∀ a ∈ 𝕌el n (A γ), t ⟨ γ ; a ⟩ ∈ 𝕌el n (B ⟨ γ ; a ⟩).
+Proof.
+  intros a Ha. apply Ht. apply setMkSigma_typing ; try assumption.
+  clear γ Hγ a Ha. intros γ Hγ. apply 𝕌el_typing. now apply HA.
+Qed.
+
 (* Telescopes (useful for labels) *)
 
 Definition typeToGraph (n : nat) (A : ZFSet) (B : ZFSet -> ZFSet) :=
   relToGraph (𝕌el n A) (𝕌 n) (HO_rel B).
 
-Definition typeTelescope2 (n : nat) (A : ZFSet -> ZFSet) (B : ZFSet -> ZFSet -> ZFSet) :=
-  fun γ => ⟨ A γ ; typeToGraph n (A γ) (B γ) ⟩. 
+Definition typeTelescope2 (n : nat) (A : ZFSet -> ZFSet) (B : ZFSet -> ZFSet) :=
+  fun γ => ⟨ A γ ; typeToGraph n (A γ) (fun a => B ⟨ γ ; a ⟩) ⟩. 
 
 Lemma typeToGraph_sorting (n : nat) {A : ZFSet} {B : ZFSet -> ZFSet} (HA : A ∈ 𝕌 n)
   (HB : ∀ a ∈ 𝕌el n A, B a ∈ 𝕌 n) : typeToGraph n A B ∈ 𝕍 n.
@@ -50,10 +110,11 @@ Proof.
   apply H1. exact H.
 Qed.
 
-Lemma typeTelescope2_typing (n : nat) {Γ : ZFSet} {A : ZFSet -> ZFSet} {B : ZFSet -> ZFSet -> ZFSet}
-  (HA : ∀ γ ∈ Γ, A γ ∈ 𝕌 n) (HB : ∀ γ ∈ Γ, ∀ a ∈ 𝕌el n (A γ), B γ a ∈ 𝕌 n) : ∀ γ ∈ Γ, typeTelescope2 n A B γ ∈ 𝕍 n.
+Lemma typeTelescope2_typing (n : nat) {Γ : ZFSet} {A : ZFSet -> ZFSet} {B : ZFSet -> ZFSet}
+  (HA : ∀ γ ∈ Γ, A γ ∈ 𝕌 n) (HB : ∀ γa ∈ ctxExt n Γ A, B γa ∈ 𝕌 n) :
+  ∀ γ ∈ Γ, typeTelescope2 n A B γ ∈ 𝕍 n.
 Proof.
   intros γ Hγ. cbn. unfold typeTelescope2. apply setMkPair_sorting.
   - apply 𝕌_incl_𝕍. now apply HA.
-  - apply typeToGraph_sorting. now apply HA. now apply HB.
+  - apply typeToGraph_sorting. now apply HA. now apply (typeExt_typing HA HB).
 Qed.
