theories/SetModel/HO_nat.v
@@ -11,9 +11,9 @@ Proof.
   + apply setMkPair_typing. apply zero_typing. apply empty_in_univ.
 Qed.
 
-Lemma natTy_HO_typing (n : nat) {γ : ZFSet} : natTy_HO γ ∈ 𝕌 n.
+Lemma natTy_HO_typing {n : nat} {Γ : ZFSet} : ∀ γ ∈ Γ, natTy_HO γ ∈ 𝕌 n.
 Proof.
-  apply setMkPair_typing.
+  intros γ Hγ. apply setMkPair_typing.
   - now apply ZFuniv_uncountable.
   - apply setMkPair_typing.
     + apply zero_typing.
@@ -33,11 +33,12 @@ Qed.
 
 (* Successor *)
 
-Definition sucTm_HO (n : nat) (t : ZFSet -> ZFSet) : ZFSet -> ZFSet :=
+Definition sucTm_HO (t : ZFSet -> ZFSet) : ZFSet -> ZFSet :=
   fun γ => ZFsuc (t γ).
 
-Lemma sucTm_HO_typing {n : nat} {Γ γ : ZFSet} {t : ZFSet -> ZFSet} (Ht : ∀ γ ∈ Γ, t γ ∈ 𝕌el n (natTy_HO γ)) (Hγ : γ ∈ Γ) :
-  sucTm_HO n t γ ∈ 𝕌el n (natTy_HO γ).
+Lemma sucTm_HO_typing {n : nat} {Γ γ : ZFSet} {t : ZFSet -> ZFSet}
+  (Ht : ∀ γ ∈ Γ, t γ ∈ 𝕌el n (natTy_HO γ)) (Hγ : γ ∈ Γ) :
+  sucTm_HO t γ ∈ 𝕌el n (natTy_HO γ).
 Proof.
   refine (transpS (fun x => _ ∈ x) _ _).
   { symmetry. apply el_natTy. }
@@ -49,16 +50,78 @@ Qed.
 
 (* Recursor *)
 
-Definition natrecTm_HO (n : nat) (P : ZFSet -> ZFSet -> ZFSet) (pz : ZFSet -> ZFSet)
-  (ps : ZFSet -> ZFSet -> ZFSet -> ZFSet) (m : ZFSet -> ZFSet) : ZFSet -> ZFSet :=
-  fun γ => natrec2 n (P γ) (pz γ) (ps γ) (m γ).
+Definition natrecTm_HO (n : nat) (P pz ps m : ZFSet -> ZFSet) : ZFSet -> ZFSet :=
+  fun γ => natrec2 n (fun m => 𝕌el n (P ⟨ γ ; m ⟩)) (pz γ) (fun m pm => ps ⟨ ⟨ γ ; m ⟩ ; pm ⟩) (m γ).
 
-(* Lemma natrecTm_HO_typing {n : nat} {Γ : ZFSet} {P : ZFSet -> ZFSet -> ZFSet} {pz : ZFSet -> ZFSet} *)
-(*   {ps : ZFSet -> ZFSet -> ZFSet -> ZFSet} {m : ZFSet -> ZFSet} *)
-(*   (HP : ∀ γ ∈ Γ, ∀ m ∈ 𝕌el n (natTy_HO γ), P γ m ∈ 𝕌 n) (Hpz : ∀ γ ∈ Γ, pz Γ ∈ P γ (zeroTm_HO γ)) *)
-(*   (Hps : ∀ γ ∈ Γ, ∀ m ∈ 𝕌el n (natTy_HO γ), ∀ pm ∈ 𝕌el n (P γ m), *)
-(*       ps γ m pm ∈ P γ (sucTm_HO n (fun γnp => ))) *)
-(*   (Hm : ∀ γ ∈ Γ, m γ ∈ 𝕌el n (natTy_HO γ)) :  *)
-(*   ∀ γ ∈ Γ, natrecTm_HO n P pz ps m ∈ 𝕌el n (P γ m). *)
+Lemma natrecTm_HO_typing_aux {n : nat} {Γ γ : ZFSet} {P ps : ZFSet -> ZFSet}
+  (HP : ∀ γm ∈ ctxExt n Γ natTy_HO, P γm ∈ 𝕌 n)
+  (Hps : ∀ γmp ∈ ctxExt n (ctxExt n Γ natTy_HO) P,
+      ps γmp ∈ 𝕌el n (P ⟨ ctx_wk n Γ natTy_HO (ctx_wk n (ctxExt n Γ natTy_HO) P γmp)
+                        ; sucTm_HO (fun γmp => ctx_var0 n Γ natTy_HO (ctx_wk n (ctxExt n Γ natTy_HO) P γmp)) γmp ⟩))
+  (Hγ : γ ∈ Γ) :
+  ∀ x ∈ ω, ∀ px ∈ 𝕌el n (P ⟨ γ ; x ⟩), ps ⟨ ⟨ γ ; x ⟩ ; px ⟩ ∈ 𝕌el n (P ⟨ γ ; ZFsuc x ⟩).
+Proof.
+  intros x Hx px Hpx.
+  assert (x ∈ 𝕌el n (natTy_HO γ)).
+  { exact (transpS (fun X => x ∈ X) (sym el_natTy) Hx). }
+  assert (⟨ ⟨ γ; x ⟩; px ⟩ ∈ ctxExt n (ctxExt n Γ natTy_HO) P) as H0.
+  { apply setMkSigma_typing ; try assumption. intros y Hy. apply 𝕌el_typing. now apply HP.
+    apply setMkSigma_typing ; try assumption. intros y Hy. apply 𝕌el_typing. now apply (natTy_HO_typing (Γ := Γ)). }
+  specialize (Hps _ H0). cbn in Hps. refine (transp2S (fun X Y => _ ∈ 𝕌el n (P ⟨ X ; Y ⟩)) _ _ Hps).
+  + refine (trans (fequal (ctx_wk n Γ natTy_HO) _) _).
+    * apply ctxExtβ1 ; try assumption. apply setMkSigma_typing ; try assumption.
+      intros y Hy. apply 𝕌el_typing. now apply (natTy_HO_typing (Γ := Γ)).
+    * apply ctxExtβ1 ; try assumption. now apply natTy_HO_typing.
+  + unfold sucTm_HO. refine (fequal ZFsuc _). refine (trans (fequal (ctx_var0 n Γ natTy_HO) _) _).
+    * apply ctxExtβ1 ; try assumption. apply setMkSigma_typing ; try assumption.
+      intros y Hy. apply 𝕌el_typing. now apply (natTy_HO_typing (Γ := Γ)).
+    * apply ctxExtβ2 ; try assumption. now apply natTy_HO_typing.
+Qed.
 
-(* Definition sucTm_HO (n : nat) (t : ZFSet -> ZFSet) : ZFSet -> ZFSet := *)
+Lemma natrecTm_HO_typing {n : nat} {Γ : ZFSet} {P pz ps m : ZFSet -> ZFSet}
+  (HP : ∀ γm ∈ ctxExt n Γ natTy_HO, P γm ∈ 𝕌 n) (Hpz : ∀ γ ∈ Γ, pz γ ∈ 𝕌el n (P ⟨ γ ; zeroTm_HO γ ⟩))
+  (Hps : ∀ γmp ∈ ctxExt n (ctxExt n Γ natTy_HO) P,
+      ps γmp ∈ 𝕌el n (P ⟨ ctx_wk n Γ natTy_HO (ctx_wk n (ctxExt n Γ natTy_HO) P γmp)
+                        ; sucTm_HO (fun γmp => ctx_var0 n Γ natTy_HO (ctx_wk n (ctxExt n Γ natTy_HO) P γmp)) γmp ⟩))
+  (Hm : ∀ γ ∈ Γ, m γ ∈ 𝕌el n (natTy_HO γ)) :
+  ∀ γ ∈ Γ, natrecTm_HO n P pz ps m γ ∈ 𝕌el n (P ⟨ γ ; m γ ⟩).
+Proof.
+  intros γ Hγ. cbn. unfold natrecTm_HO. apply (natrec2_typing (P := fun m => 𝕌el n (P ⟨ γ ; m ⟩))).
+  - intros x Hx. apply 𝕌el_typing. apply (typeExt_typing natTy_HO_typing HP). assumption.
+    exact (transpS (fun X => x ∈ X) (sym el_natTy) Hx).
+  - now apply Hpz.
+  - now apply (natrecTm_HO_typing_aux HP Hps Hγ).
+  - exact (transpS (fun X => m γ ∈ X) el_natTy (Hm γ Hγ)).
+Qed.
+
+Lemma natrecTm_HO_β1 {n : nat} {Γ : ZFSet} {P pz ps : ZFSet -> ZFSet}
+  (HP : ∀ γm ∈ ctxExt n Γ natTy_HO, P γm ∈ 𝕌 n) (Hpz : ∀ γ ∈ Γ, pz γ ∈ 𝕌el n (P ⟨ γ ; zeroTm_HO γ ⟩))
+  (Hps : ∀ γmp ∈ ctxExt n (ctxExt n Γ natTy_HO) P,
+      ps γmp ∈ 𝕌el n (P ⟨ ctx_wk n Γ natTy_HO (ctx_wk n (ctxExt n Γ natTy_HO) P γmp)
+                        ; sucTm_HO (fun γmp => ctx_var0 n Γ natTy_HO (ctx_wk n (ctxExt n Γ natTy_HO) P γmp)) γmp ⟩)) :
+  ∀ γ ∈ Γ, natrecTm_HO n P pz ps zeroTm_HO γ ≡ pz γ.
+Proof.
+  intros γ Hγ. cbn. unfold natrecTm_HO. unfold zeroTm_HO. apply natrec2_β1.
+  - intros x Hx. apply 𝕌el_typing. apply (typeExt_typing natTy_HO_typing HP). assumption.
+    exact (transpS (fun X => x ∈ X) (sym el_natTy) Hx).
+  - now apply Hpz.
+  - now apply (natrecTm_HO_typing_aux HP Hps Hγ).
+Qed.
+
+Lemma natrecTm_HO_β2 {n : nat} {Γ : ZFSet} {P pz ps m : ZFSet -> ZFSet}
+  (HP : ∀ γm ∈ ctxExt n Γ natTy_HO, P γm ∈ 𝕌 n) (Hpz : ∀ γ ∈ Γ, pz γ ∈ 𝕌el n (P ⟨ γ ; zeroTm_HO γ ⟩))
+  (Hps : ∀ γmp ∈ ctxExt n (ctxExt n Γ natTy_HO) P,
+      ps γmp ∈ 𝕌el n (P ⟨ ctx_wk n Γ natTy_HO (ctx_wk n (ctxExt n Γ natTy_HO) P γmp)
+                        ; sucTm_HO (fun γmp => ctx_var0 n Γ natTy_HO (ctx_wk n (ctxExt n Γ natTy_HO) P γmp)) γmp ⟩))
+  (Hm : ∀ γ ∈ Γ, m γ ∈ 𝕌el n (natTy_HO γ)) :
+  ∀ γ ∈ Γ, natrecTm_HO n P pz ps (sucTm_HO m) γ ≡ ps ⟨ ⟨ γ ; m γ ⟩ ; natrecTm_HO n P pz ps m γ ⟩.
+Proof.
+  intros γ Hγ. cbn. unfold natrecTm_HO. unfold sucTm_HO. refine (trans _ _).
+  - apply natrec2_β2.
+    + intros x Hx. apply 𝕌el_typing. apply (typeExt_typing natTy_HO_typing HP). assumption.
+      exact (transpS (fun X => x ∈ X) (sym el_natTy) Hx).
+    + now apply Hpz.
+    + now apply (natrecTm_HO_typing_aux HP Hps Hγ).
+    + exact (transpS (fun X => m γ ∈ X) el_natTy (Hm γ Hγ)).
+  - reflexivity.
+Qed.
