theories/SetModel/HO_pi.v
@@ -4,46 +4,46 @@ Require Import HO.
 
 (* Pi types *)
 
-Definition piTy_HO (n : nat) (A : ZFSet -> ZFSet) (B : ZFSet -> ZFSet -> ZFSet) : ZFSet -> ZFSet :=
-  fun γ => ⟨ setPi n (𝕌el n (A γ)) (fun a => 𝕌el n (B γ a))
+Definition piTy_HO (n : nat) (A : ZFSet -> ZFSet) (B : ZFSet -> ZFSet) : ZFSet -> ZFSet :=
+  fun γ => ⟨ setPi n (𝕌el n (A γ)) (fun a => 𝕌el n (B ⟨ γ ; a ⟩))
            ; ⟨ ZFone ; typeTelescope2 n A B γ ⟩ ⟩.
 
-Lemma piTy_HO_typing (n : nat) {Γ : ZFSet} {A : ZFSet -> ZFSet} {B : ZFSet -> ZFSet -> ZFSet}
-  (HA : ∀ γ ∈ Γ, A γ ∈ 𝕌 n) (HB : ∀ γ ∈ Γ, ∀ a ∈ 𝕌el n (A γ), B γ a ∈ 𝕌 n) :
+Lemma piTy_HO_typing {n : nat} {Γ : ZFSet} {A : ZFSet -> ZFSet} {B : ZFSet -> ZFSet}
+  (HA : ∀ γ ∈ Γ, A γ ∈ 𝕌 n) (HB : ∀ γa ∈ ctxExt n Γ A, B γa ∈ 𝕌 n) :
   ∀ γ ∈ Γ, piTy_HO n A B γ ∈ 𝕌 n.
 Proof.
   intros γ Hγ. cbn. apply setMkPair_typing.
   - apply setPi_typing.
     + apply 𝕌el_typing. now apply HA.
-    + intros a Ha. apply 𝕌el_typing. now apply HB. 
+    + intros a Ha. apply 𝕌el_typing. now apply (typeExt_typing HA HB). 
   - apply setMkPair_typing.
     + apply one_typing.
-    + now apply (typeTelescope2_typing n (Γ := Γ)).
+    + apply (typeTelescope2_typing n (Γ := Γ)) ; try assumption. 
 Qed.
 
-Lemma el_piTy {n : nat} {Γ γ : ZFSet} {A : ZFSet -> ZFSet} {B : ZFSet -> ZFSet -> ZFSet}
-  (HA : ∀ γ ∈ Γ, A γ ∈ 𝕌 n) (HB : ∀ γ ∈ Γ, ∀ a ∈ 𝕌el n (A γ), B γ a ∈ 𝕌 n) (Hγ : γ ∈ Γ) :
-  𝕌el n (piTy_HO n A B γ) ≡ setPi n (𝕌el n (A γ)) (fun a => 𝕌el n (B γ a)).
+Lemma el_piTy {n : nat} {Γ γ : ZFSet} {A : ZFSet -> ZFSet} {B : ZFSet -> ZFSet}
+  (HA : ∀ γ ∈ Γ, A γ ∈ 𝕌 n) (HB : ∀ γa ∈ ctxExt n Γ A, B γa ∈ 𝕌 n) (Hγ : γ ∈ Γ) :
+  𝕌el n (piTy_HO n A B γ) ≡ setPi n (𝕌el n (A γ)) (fun a => 𝕌el n (B ⟨ γ ; a ⟩)).
 Proof.
-  apply setPairβ1'. now apply (piTy_HO_typing n (Γ := Γ)).
+  apply setPairβ1'. now apply (piTy_HO_typing (Γ := Γ)).
 Qed.
 
-Lemma hd_piTy {n : nat} {Γ γ : ZFSet} {A : ZFSet -> ZFSet} {B : ZFSet -> ZFSet -> ZFSet}
-  (HA : ∀ γ ∈ Γ, A γ ∈ 𝕌 n) (HB : ∀ γ ∈ Γ, ∀ a ∈ 𝕌el n (A γ), B γ a ∈ 𝕌 n) (Hγ : γ ∈ Γ) :
+Lemma hd_piTy {n : nat} {Γ γ : ZFSet} {A : ZFSet -> ZFSet} {B : ZFSet -> ZFSet}
+  (HA : ∀ γ ∈ Γ, A γ ∈ 𝕌 n) (HB : ∀ γa ∈ ctxExt n Γ A, B γa ∈ 𝕌 n) (Hγ : γ ∈ Γ) :
   𝕌hd n (piTy_HO n A B γ) ≡ ZFone.
 Proof.
   refine (trans (fequal (setFstPair ω (𝕍 n)) _) _).
-  apply setPairβ2'. now apply (piTy_HO_typing n (Γ := Γ)).
-  apply setPairβ1. apply one_typing. now apply (typeTelescope2_typing n (Γ := Γ)).
+  apply setPairβ2'. now apply (piTy_HO_typing (Γ := Γ)).
+  apply setPairβ1. apply one_typing. apply (typeTelescope2_typing n (Γ := Γ)) ; try assumption.
 Qed.  
 
-Lemma lbl_piTy {n : nat} {Γ γ : ZFSet} {A : ZFSet -> ZFSet} {B : ZFSet -> ZFSet -> ZFSet}
-  (HA : ∀ γ ∈ Γ, A γ ∈ 𝕌 n) (HB : ∀ γ ∈ Γ, ∀ a ∈ 𝕌el n (A γ), B γ a ∈ 𝕌 n) (Hγ : γ ∈ Γ) :
+Lemma lbl_piTy {n : nat} {Γ γ : ZFSet} {A : ZFSet -> ZFSet} {B : ZFSet -> ZFSet}
+  (HA : ∀ γ ∈ Γ, A γ ∈ 𝕌 n) (HB : ∀ γa ∈ ctxExt n Γ A, B γa ∈ 𝕌 n) (Hγ : γ ∈ Γ) :
   𝕌lbl n (piTy_HO n A B γ) ≡ typeTelescope2 n A B γ.
 Proof.
   refine (trans (fequal (setSndPair ω (𝕍 n)) _) _).
-  apply setPairβ2'. now apply (piTy_HO_typing n (Γ := Γ)).
-  apply setPairβ2. apply one_typing. now apply (typeTelescope2_typing n (Γ := Γ)).
+  apply setPairβ2'. now apply (piTy_HO_typing (Γ := Γ)).
+  apply setPairβ2. apply one_typing. apply (typeTelescope2_typing n (Γ := Γ)) ; try assumption.
 Qed.
 
 (* Injectivity of Pi types *)
@@ -54,27 +54,27 @@ Definition dom_piTy (n : nat) (x : ZFSet) :=
 Definition cod_piTy (n : nat) (x : ZFSet) :=
   setSndPair (𝕌 n) (𝕍 n) (𝕌lbl n x).
 
-Lemma dom_piTy_eq {n : nat} {Γ γ : ZFSet} {A : ZFSet -> ZFSet} {B : ZFSet -> ZFSet -> ZFSet}
-  (HA : ∀ γ ∈ Γ, A γ ∈ 𝕌 n) (HB : ∀ γ ∈ Γ, ∀ a ∈ 𝕌el n (A γ), B γ a ∈ 𝕌 n) (Hγ : γ ∈ Γ) :
+Lemma dom_piTy_eq {n : nat} {Γ γ : ZFSet} {A : ZFSet -> ZFSet} {B : ZFSet -> ZFSet}
+  (HA : ∀ γ ∈ Γ, A γ ∈ 𝕌 n) (HB : ∀ γa ∈ ctxExt n Γ A, B γa ∈ 𝕌 n) (Hγ : γ ∈ Γ) :
   dom_piTy n (piTy_HO n A B γ) ≡ A γ.
 Proof.
   refine (trans (fequal (setFstPair (𝕌 n) (𝕍 n)) _) _).
   now apply (lbl_piTy (Γ := Γ)). apply setPairβ1. now apply HA.
-  apply typeToGraph_sorting. now apply HA. now apply HB.
+  apply typeToGraph_sorting. now apply HA. now apply (typeExt_typing HA HB).
 Qed.
 
-Lemma cod_piTy_eq {n : nat} {Γ γ : ZFSet} {A : ZFSet -> ZFSet} {B : ZFSet -> ZFSet -> ZFSet}
-  (HA : ∀ γ ∈ Γ, A γ ∈ 𝕌 n) (HB : ∀ γ ∈ Γ, ∀ a ∈ 𝕌el n (A γ), B γ a ∈ 𝕌 n) (Hγ : γ ∈ Γ) :
-  cod_piTy n (piTy_HO n A B γ) ≡ typeToGraph n (A γ) (B γ).
+Lemma cod_piTy_eq {n : nat} {Γ γ : ZFSet} {A : ZFSet -> ZFSet} {B : ZFSet -> ZFSet}
+  (HA : ∀ γ ∈ Γ, A γ ∈ 𝕌 n) (HB : ∀ γa ∈ ctxExt n Γ A, B γa ∈ 𝕌 n) (Hγ : γ ∈ Γ) :
+  cod_piTy n (piTy_HO n A B γ) ≡ typeToGraph n (A γ) (fun a => B ⟨ γ ; a ⟩).
 Proof.
   refine (trans (fequal (setSndPair (𝕌 n) (𝕍 n)) _) _).
   now apply (lbl_piTy (Γ := Γ)). apply setPairβ2. now apply HA.
-  apply typeToGraph_sorting. now apply HA. now apply HB.
+  apply typeToGraph_sorting. now apply HA. now apply (typeExt_typing HA HB).
 Qed.
 
-Lemma piTy_HO_inj1 (n : nat) {Γ γ : ZFSet} {A A' : ZFSet -> ZFSet} {B B' : ZFSet -> ZFSet -> ZFSet}
-  (HA : ∀ γ ∈ Γ, A γ ∈ 𝕌 n) (HB : ∀ γ ∈ Γ, ∀ a ∈ 𝕌el n (A γ), B γ a ∈ 𝕌 n)
-  (HA' : ∀ γ ∈ Γ, A' γ ∈ 𝕌 n) (HB' : ∀ γ ∈ Γ, ∀ a ∈ 𝕌el n (A' γ), B' γ a ∈ 𝕌 n)
+Lemma piTy_HO_inj1 {n : nat} {Γ γ : ZFSet} {A A' B B' : ZFSet -> ZFSet} 
+  (HA : ∀ γ ∈ Γ, A γ ∈ 𝕌 n) (HB : ∀ γa ∈ ctxExt n Γ A, B γa ∈ 𝕌 n)
+  (HA' : ∀ γ ∈ Γ, A' γ ∈ 𝕌 n) (HB' : ∀ γa ∈ ctxExt n Γ A', B' γa ∈ 𝕌 n)
   (Hγ : γ ∈ Γ) (H : piTy_HO n A B γ ≡ piTy_HO n A' B' γ) : A γ ≡ A' γ.
 Proof.
   refine (trans (b := dom_piTy n (piTy_HO n A B γ)) _ _).
@@ -82,66 +82,68 @@ Proof.
   refine (trans (fequal (dom_piTy n) H) _). now apply (dom_piTy_eq (Γ := Γ)).
 Qed.
 
-Lemma piTy_HO_inj2' (n : nat) {Γ γ : ZFSet} {A A' : ZFSet -> ZFSet} {B B' : ZFSet -> ZFSet -> ZFSet}
-  (HA : ∀ γ ∈ Γ, A γ ∈ 𝕌 n) (HB : ∀ γ ∈ Γ, ∀ a ∈ 𝕌el n (A γ), B γ a ∈ 𝕌 n)
-  (HA' : ∀ γ ∈ Γ, A' γ ∈ 𝕌 n) (HB' : ∀ γ ∈ Γ, ∀ a ∈ 𝕌el n (A' γ), B' γ a ∈ 𝕌 n)
+Lemma piTy_HO_inj2' {n : nat} {Γ γ : ZFSet} {A A' B B' : ZFSet -> ZFSet} 
+  (HA : ∀ γ ∈ Γ, A γ ∈ 𝕌 n) (HB : ∀ γa ∈ ctxExt n Γ A, B γa ∈ 𝕌 n)
+  (HA' : ∀ γ ∈ Γ, A' γ ∈ 𝕌 n) (HB' : ∀ γa ∈ ctxExt n Γ A', B' γa ∈ 𝕌 n)
   (Hγ : γ ∈ Γ) (H : piTy_HO n A B γ ≡ piTy_HO n A' B' γ) :
-  typeToGraph n (A γ) (B γ) ≡ typeToGraph n (A γ) (B' γ).
+  typeToGraph n (A γ) (fun a => B ⟨ γ ; a ⟩) ≡ typeToGraph n (A γ) (fun a => B' ⟨ γ ; a ⟩).
 Proof.
-  pose proof (piTy_HO_inj1 n HA HB HA' HB' Hγ H) as HAA'.
+  pose proof (piTy_HO_inj1 HA HB HA' HB' Hγ H) as HAA'.
   refine (trans (b := cod_piTy n (piTy_HO n A B γ)) _ _).
   symmetry. now apply (cod_piTy_eq (Γ := Γ)). refine (trans (fequal (cod_piTy n) H) _).
-  refine (transpS (fun X => _ ≡ typeToGraph n X (B' γ)) (sym HAA') _).
+  refine (transpS (fun X => _ ≡ typeToGraph n X _) (sym HAA') _).
   now apply (cod_piTy_eq (Γ := Γ)).
 Qed.
 
-Lemma piTy_HO_inj2 (n : nat) {Γ γ a : ZFSet} {A A' : ZFSet -> ZFSet} {B B' : ZFSet -> ZFSet -> ZFSet}
-  (HA : ∀ γ ∈ Γ, A γ ∈ 𝕌 n) (HB : ∀ γ ∈ Γ, ∀ a ∈ 𝕌el n (A γ), B γ a ∈ 𝕌 n)
-  (HA' : ∀ γ ∈ Γ, A' γ ∈ 𝕌 n) (HB' : ∀ γ ∈ Γ, ∀ a ∈ 𝕌el n (A' γ), B' γ a ∈ 𝕌 n)
+Lemma piTy_HO_inj2 {n : nat} {Γ γ a : ZFSet} {A A' B B' : ZFSet -> ZFSet} 
+  (HA : ∀ γ ∈ Γ, A γ ∈ 𝕌 n) (HB : ∀ γa ∈ ctxExt n Γ A, B γa ∈ 𝕌 n)
+  (HA' : ∀ γ ∈ Γ, A' γ ∈ 𝕌 n) (HB' : ∀ γa ∈ ctxExt n Γ A', B' γa ∈ 𝕌 n)
   (Hγ : γ ∈ Γ) (H : piTy_HO n A B γ ≡ piTy_HO n A' B' γ) (Ha : a ∈ 𝕌el n (A γ)) :
-  B γ a ≡ B' γ a.
+  B ⟨ γ ; a ⟩ ≡ B' ⟨ γ ; a ⟩.
 Proof.
-  pose proof (piTy_HO_inj1 n HA HB HA' HB' Hγ H) as HAA'.
-  pose proof (piTy_HO_inj2' n HA HB HA' HB' Hγ H) as HBB'.
-  refine (trans (b := setAppArr (𝕌el n (A γ)) (𝕌 n) (typeToGraph n (A γ) (B γ)) a) _ _).
-  { symmetry. apply setAppArr_HO. intros a' Ha'. now apply HB. assumption. }
+  pose proof (piTy_HO_inj1 HA HB HA' HB' Hγ H) as HAA'.
+  pose proof (piTy_HO_inj2' HA HB HA' HB' Hγ H) as HBB'.
+  refine (trans (b := setAppArr (𝕌el n (A γ)) (𝕌 n) (typeToGraph n (A γ) (fun a => B ⟨ γ ; a ⟩)) a) _ _).
+  { symmetry. refine (trans _ _). apply setAppArr_HO ; try assumption.
+    now apply (typeExt_typing HA HB). reflexivity. }
   refine (trans (fequal (fun X => setAppArr (𝕌el n (A γ)) (𝕌 n) X a) HBB') _).
-  apply setAppArr_HO. intros a' Ha'. apply HB' ; try assumption.
-  refine (transpS (fun X => a' ∈ 𝕌el n X) HAA' _). assumption. assumption.
+  refine (trans _ _). apply setAppArr_HO ; try assumption. 2:reflexivity.
+  intros a' Ha'. pose proof (transpS (fun X => a' ∈ 𝕌el n X) HAA' Ha') as Ha''. cbn in Ha''. clear Ha'.
+  revert a' Ha''. now apply (typeExt_typing HA' HB').
 Qed.
 
 (* Lambda abstraction *)
 
-Definition lamTm_HO (n : nat) (A : ZFSet -> ZFSet) 
-  (t : ZFSet -> ZFSet -> ZFSet) : ZFSet -> ZFSet :=
-  fun γ => relToGraph (𝕌el n (A γ)) (𝕍 n) (HO_rel (t γ)).
+Definition lamTm_HO (n : nat) (A t : ZFSet -> ZFSet) : ZFSet -> ZFSet :=
+  fun γ => relToGraph (𝕌el n (A γ)) (𝕍 n) (HO_rel (fun a => t ⟨ γ ; a ⟩)).
 
-Lemma lamTm_HO_typing (n : nat) {Γ : ZFSet} {A : ZFSet -> ZFSet} {B : ZFSet -> ZFSet -> ZFSet}
-  {t : ZFSet -> ZFSet -> ZFSet} (HA : ∀ γ ∈ Γ, A γ ∈ 𝕌 n) (HB : ∀ γ ∈ Γ, ∀ a ∈ 𝕌el n (A γ), B γ a ∈ 𝕌 n)
-  (Ht : ∀ γ ∈ Γ, ∀ a ∈ 𝕌el n (A γ), t γ a ∈ 𝕌el n (B γ a)) :
+Lemma lamTm_HO_typing (n : nat) {Γ : ZFSet} {A B t : ZFSet -> ZFSet}
+  (HA : ∀ γ ∈ Γ, A γ ∈ 𝕌 n) (HB : ∀ γa ∈ ctxExt n Γ A, B γa ∈ 𝕌 n)
+  (Ht : ∀ γa ∈ ctxExt n Γ A, t γa ∈ 𝕌el n (B γa)) :
   ∀ γ ∈ Γ, lamTm_HO n A t γ ∈ 𝕌el n (piTy_HO n A B γ).
 Proof.
-  intros γ Hγ. cbn. refine (transpS (fun X => _ ∈ X) (sym (el_piTy HA HB Hγ)) _).
-  apply ZFincomp. split.
-  - apply relToGraph_typing. apply HO_rel_typing. intros a Ha.
-    eapply ZFuniv_trans. now apply Ht. apply 𝕌el_typing. now apply HB.
-  - intros a Ha. refine (transpS (fun X => X ∈ 𝕌el n (B γ a)) _ (Ht γ Hγ a Ha)).
-    refine (sym _). apply setAppArr_HO ; [ | assumption].
-    intros a' Ha'. eapply ZFuniv_trans. now apply Ht. apply 𝕌el_typing. now apply HB.
+  intros γ Hγ. cbn. refine (transpS (fun X => _ ∈ X) (sym (el_piTy HA HB Hγ)) _). apply ZFincomp. split.
+  - apply relToGraph_typing. apply HO_rel_typing.
+    intros a Ha. eapply ZFuniv_trans. now apply (termExt_typing HA HB Ht).
+    apply 𝕌el_typing. now apply (typeExt_typing HA HB).
+  - intros a Ha. refine (transpS (fun X => X ∈ 𝕌el n (B ⟨ γ ; a ⟩)) _ (Ht ⟨ γ ; a ⟩ _)).
+    + refine (sym _). refine (trans _ _). apply setAppArr_HO ; [ | assumption].
+      intros a' Ha'. eapply ZFuniv_trans. now apply (termExt_typing HA HB Ht). apply 𝕌el_typing.
+      now apply (typeExt_typing HA HB). reflexivity.
+    + apply setMkSigma_typing ; try assumption. intros γ' Hγ'. apply 𝕌el_typing. now apply HA.
 Qed.
 
 (* Application *)
 
-Definition appTm_HO (n : nat) (A : ZFSet -> ZFSet) 
-  (t : ZFSet -> ZFSet) (u : ZFSet -> ZFSet) : ZFSet -> ZFSet :=
+Definition appTm_HO (n : nat) (A t u : ZFSet -> ZFSet) : ZFSet -> ZFSet :=
   fun γ => setAppArr (𝕌el n (A γ)) (𝕍 n) (t γ) (u γ).
 
-Lemma appTm_HO_typing (n : nat) {Γ : ZFSet} {A : ZFSet -> ZFSet} {B : ZFSet -> ZFSet -> ZFSet}
-  {t u : ZFSet -> ZFSet} (HA : ∀ γ ∈ Γ, A γ ∈ 𝕌 n) (HB : ∀ γ ∈ Γ, ∀ a ∈ 𝕌el n (A γ), B γ a ∈ 𝕌 n)
+Lemma appTm_HO_typing (n : nat) {Γ : ZFSet} {A B t u : ZFSet -> ZFSet} 
+  (HA : ∀ γ ∈ Γ, A γ ∈ 𝕌 n) (HB : ∀ γa ∈ ctxExt n Γ A, B γa ∈ 𝕌 n)
   (Ht : ∀ γ ∈ Γ, t γ ∈ 𝕌el n (piTy_HO n A B γ)) (Hu : ∀ γ ∈ Γ, u γ ∈ 𝕌el n (A γ)) :
-  ∀ γ ∈ Γ, appTm_HO n A t u γ ∈ 𝕌el n (B γ (u γ)).
+  ∀ γ ∈ Γ, appTm_HO n A t u γ ∈ 𝕌el n (B ⟨ γ ; u γ ⟩).
 Proof.
-  intros γ Hγ. assert (t γ ∈ setPi n (𝕌el n (A γ)) (fun a => 𝕌el n (B γ a))) as Htγ.
+  intros γ Hγ. assert (t γ ∈ setPi n (𝕌el n (A γ)) (fun a => 𝕌el n (B ⟨ γ ; a ⟩))) as Htγ.
   { refine (transpS (fun X => t γ ∈ X) _ (Ht γ Hγ)). now apply (el_piTy (Γ := Γ)). }
   cbn. unfold appTm_HO. apply ZFincomp in Htγ. destruct Htγ as [ _ H ].
   apply H. now apply Hu.
@@ -149,30 +151,44 @@ Qed.
 
 (* Equations (β and η) *)
 
-Lemma piTy_HO_β (n : nat) {Γ : ZFSet} {A u : ZFSet -> ZFSet} {B t : ZFSet -> ZFSet -> ZFSet}
-  (HA : ∀ γ ∈ Γ, A γ ∈ 𝕌 n) (HB : ∀ γ ∈ Γ, ∀ a ∈ 𝕌el n (A γ), B γ a ∈ 𝕌 n)
-  (Ht : ∀ γ ∈ Γ, ∀ a ∈ 𝕌el n (A γ), t γ a ∈ 𝕌el n (B γ a)) (Hu : ∀ γ ∈ Γ, u γ ∈ 𝕌el n (A γ)) :
-  ∀ γ ∈ Γ, appTm_HO n A (lamTm_HO n A t) u γ ≡ t γ (u γ).
+Lemma piTy_HO_β (n : nat) {Γ : ZFSet} {A B t u : ZFSet -> ZFSet} 
+  (HA : ∀ γ ∈ Γ, A γ ∈ 𝕌 n) (HB : ∀ γa ∈ ctxExt n Γ A, B γa ∈ 𝕌 n)
+  (Ht : ∀ γa ∈ ctxExt n Γ A, t γa ∈ 𝕌el n (B γa)) (Hu : ∀ γ ∈ Γ, u γ ∈ 𝕌el n (A γ)) :
+  ∀ γ ∈ Γ, appTm_HO n A (lamTm_HO n A t) u γ ≡ t ⟨ γ ; u γ ⟩.
 Proof.
-  intros γ Hγ. cbn. apply setAppArr_HO.
-  - intros a Ha. eapply ZFuniv_trans. now apply Ht. apply 𝕌el_typing. now apply HB.
+  intros γ Hγ. cbn. refine (trans _ _). apply setAppArr_HO ; try assumption. 3:reflexivity.
+  - intros a Ha. eapply ZFuniv_trans. now apply (termExt_typing HA HB Ht). apply 𝕌el_typing.
+    now apply (typeExt_typing HA HB).
   - now apply Hu.
 Qed.
 
-Lemma piTy_HO_η (n : nat) {Γ : ZFSet} {A t : ZFSet -> ZFSet} {B : ZFSet -> ZFSet -> ZFSet}
-  (HA : ∀ γ ∈ Γ, A γ ∈ 𝕌 n) (HB : ∀ γ ∈ Γ, ∀ a ∈ 𝕌el n (A γ), B γ a ∈ 𝕌 n)
+(* Γ ⊢ t : Π A B *)
+
+(* Γ , A ⊢ wk t : Π (wk A) (wk1 B) *)
+(* Γ , A ⊢ 0 : wk A *)
+(* Γ , A ⊢ (wk t) @ 0 : wk1 B [ 0 ] = B *)
+(* Γ ⊢ λ (wk t) @ 0 : Π A B *)
+
+Lemma piTy_HO_η (n : nat) {Γ : ZFSet} {A B t u : ZFSet -> ZFSet}
+  (HA : ∀ γ ∈ Γ, A γ ∈ 𝕌 n) (HB : ∀ γa ∈ ctxExt n Γ A, B γa ∈ 𝕌 n)
   (Ht : ∀ γ ∈ Γ, t γ ∈ 𝕌el n (piTy_HO n A B γ)) :
-  ∀ γ ∈ Γ, t γ ≡ lamTm_HO n A (fun γ a => appTm_HO n A t (fun γ => a) γ) γ.
+  ∀ γ ∈ Γ, t γ ≡ lamTm_HO n A (fun γa => appTm_HO n (fun γa => A (ctx_wk n Γ A γa)) (fun γa => t (ctx_wk n Γ A γa)) (ctx_var0 n Γ A) γa) γ.
 Proof.
   intros γ Hγ. cbn. unfold lamTm_HO. unfold appTm_HO.
-  assert (t γ ∈ setPi n (𝕌el n (A γ)) (fun a => 𝕌el n (B γ a))) as Ht'.
+  assert (t γ ∈ setPi n (𝕌el n (A γ)) (fun a => 𝕌el n (B ⟨ γ ; a ⟩))) as Ht'.
   { refine (transpS (fun X => t γ ∈ X) (el_piTy HA HB Hγ) _). now apply Ht. }
   apply ZFincomp in Ht'. destruct Ht' as [ Ht' _ ].
-  change (fun a : ZFSet => setAppArr (𝕌el n (A γ)) (𝕍 n) (t γ) a) with (setAppArr (𝕌el n (A γ)) (𝕍 n) (t γ)).
   apply (setArr_funext (A := 𝕌el n (A γ)) (B := 𝕍 n)).
   - exact Ht'.
-  - apply relToGraph_typing. apply HO_rel_typing.
-    intros a Ha. apply setAppArr_typing. 2:assumption. exact Ht'.
-  - intros a Ha. refine (sym _). apply setAppArr_HO. 2:assumption. clear a Ha.
-    intros a Ha. apply setAppArr_typing. 2:assumption. exact Ht'.
+  - apply relToGraph_typing. apply HO_rel_typing. intros a Ha.
+    refine (transp2S (fun X Y => setAppArr (𝕌el n (A X)) (𝕍 n) (t X) Y ∈ 𝕍 n)
+              (sym (ctxExtβ1 HA Hγ Ha)) (sym (ctxExtβ2 HA Hγ Ha)) _).
+    apply setAppArr_typing. 2:assumption. exact Ht'.
+  - intros a Ha. refine (sym _). refine (trans _ _). apply setAppArr_HO. 2:assumption.
+    + clear a Ha. intros a Ha. 
+      refine (transp2S (fun X Y => setAppArr (𝕌el n (A X)) (𝕍 n) (t X) Y ∈ 𝕍 n)
+                (sym (ctxExtβ1 HA Hγ Ha)) (sym (ctxExtβ2 HA Hγ Ha)) _).
+      apply setAppArr_typing. 2:assumption. exact Ht'.
+    + refine (fequal2 (fun X Y => setAppArr (𝕌el n (A X)) (𝕍 n) (t X) Y)
+                ((ctxExtβ1 HA Hγ Ha)) ((ctxExtβ2 HA Hγ Ha))).
 Qed.
